implement lifting of boolean connectives
the expression lifter is now able to lift expressions like "bool2b (b1
/\ b2". This required reasoning about the boolean values of immediate
expressions. This is a rather large addition:

- new theory bir_bool_exp added to reason about boolean immediate
expressions
- new evaluation `bir_eval_bool_exp` introduced
- guard `bir_is_bool_exp_env` introduced
- `bir_env_var_is_initialised` extended to deal with type of vars
- `bir_env_order` adapted to reflect change in
`bir_env_var_is_initialised`
- we could in theorem `type_of_bir_exp_THM_with_init_vars` get rid of
precondition ``bir_is_well_typed_env env` after the strengthening of
`bir_env_var_is_initialised`

src/tools/bir_exp_liftingLib.sml
@@ -488,6 +488,11 @@ bir_exp_lift env_t n ``(Imm16 (sw2sw (7w:word8)))``
 bir_exp_lift env_t n ``Imm32 (w2w ((v2w [F; F; F; F; T; F; F]):word8))``
 bir_exp_lift env_t n ``Imm32 (w2w ((v2w [F; F; F; F; T; F; F]):word7))``
 
+bir_exp_lift env_t n ``(w1:word32 < w2) /\ (w2 < w3)``
+bir_exp_lift env_t n ``(w1:word32 < w2) \/ (w2 < w3)``
+bir_exp_lift env_t n ``(w1:word32 < w2) ==> (w2 < w3)``
+
+
 bir_exp_lift env_t n ``if (w1:word32 < w2) then 0w:word16 else 16w``
 
 bir_exp_lift env_t n ``Imm32((((mem:word32 -> word8)
