src/core-props/bir_bool_expScript.sml
@@ -1,0 +1,487 @@
+open HolKernel Parse boolLib bossLib;
+open bir_envTheory bir_valuesTheory;
+open bir_immTheory bir_typing_expTheory;
+open bir_mem_expTheory bir_expTheory;
+open bir_imm_expTheory;
+open HolBACoreSimps
+
+val _ = new_theory "bir_bool_exp";
+
+
+(******************)
+(* boolean values *)
+(******************)
+
+val bir_val_true_def  = Define `bir_val_true  = BVal_Imm   (Imm1 1w)`;
+val bir_val_false_def = Define `bir_val_false = BVal_Imm   (Imm1 0w)`;
+
+val bir_val_TF_dist = store_thm ("bir_val_TF_dist",
+  ``(bir_val_false <> bir_val_true)``,
+SIMP_TAC (std_ss ++ holBACore_ss ++ wordsLib.WORD_ss) [bir_val_false_def, bir_val_true_def]);
+
+
+val type_of_bir_val_TF = store_thm ("type_of_bir_val_TF",
+  ``(type_of_bir_val bir_val_true = SOME BType_Bool) /\
+    (type_of_bir_val bir_val_false = SOME BType_Bool)``,
+
+SIMP_TAC (std_ss++holBACore_ss) [bir_val_false_def, bir_val_true_def,
+  BType_Bool_def]);
+
+
+val bir_val_is_Bool_ALT_DEF = store_thm ("bir_val_is_Bool_ALT_DEF",
+``!v. bir_val_is_Bool v <=> ((v = bir_val_false) \/ (v = bir_val_true))``,
+
+SIMP_TAC (std_ss++holBACore_ss) [bir_val_is_Bool_def,
+  bir_val_is_Imm_s_def, bir_val_true_def, bir_val_false_def] >>
+REPEAT STRIP_TAC >> EQ_TAC >> STRIP_TAC >| [
+  Cases_on `(n2w n):word1` >>
+  Cases_on `(n'=0) \/ (n'=1)` >- METIS_TAC[] >>
+  FULL_SIMP_TAC (arith_ss++wordsLib.WORD_ss) [],
+
+  METIS_TAC[],
+  METIS_TAC[]
+]);
+
+
+val bir_dest_bool_val_TF = store_thm ("bir_dest_bool_val_TF",
+  ``((bir_dest_bool_val bir_val_false) = SOME F) /\
+    ((bir_dest_bool_val bir_val_true) = SOME T)``,
+
+SIMP_TAC (std_ss++wordsLib.WORD_ss) [bir_val_false_def, bir_val_true_def, bir_dest_bool_val_def]);
+
+
+val bool2w_ELIMS = store_thm ("bool2w_ELIMS",
+  ``(!b. ((bool2w b = 0w) <=> ~b)) /\
+    (!b. ((bool2w b = 1w) <=> b)) /\
+    (!b1 b2. (bool2w b1 = bool2w b2) <=> (b1 = b2))``,
+
+SIMP_TAC (std_ss++holBACore_ss++boolSimps.LIFT_COND_ss++
+  wordsLib.WORD_ss) [bool2w_def]);
+
+
+val bool2b_ELIMS = store_thm ("bool2b_ELIMS",
+  ``(!b w. ((bool2b b = Imm1 w) <=> (bool2w b = w))) /\
+    (!b1 b2. (bool2b b1 = bool2b b2) <=> (b1 = b2))``,
+
+SIMP_TAC (std_ss++holBACore_ss++boolSimps.LIFT_COND_ss) [bool2b_def, bool2w_ELIMS]);
+
+
+val bir_val_is_Bool_bool2b = store_thm ("bir_val_is_Bool_bool2b",
+  ``!b. bir_val_is_Bool (BVal_Imm (bool2b b))``,
+SIMP_TAC (std_ss++holBACore_ss) [bir_val_is_Bool_ALT_DEF]);
+
+
+val bir_mk_bool_val_def = Define `bir_mk_bool_val b = BVal_Imm (bool2b b)`;
+
+val bir_mk_bool_val_is_bool = store_thm ("bir_mk_bool_val_is_bool",
+  ``!b. bir_val_is_Bool (bir_mk_bool_val b)``,
+SIMP_TAC std_ss [bir_mk_bool_val_def, bir_val_is_Bool_bool2b]);
+
+
+val bir_mk_bool_val_ALT_DEF_TF = store_thm ("bir_mk_bool_val_ALT_DEF_TF",
+  ``!b. bir_mk_bool_val b = (if b then bir_val_true else bir_val_false)``,
+SIMP_TAC (std_ss++boolSimps.LIFT_COND_ss) [bir_mk_bool_val_def, bool2b_def, bir_val_true_def, bir_val_false_def, bool2w_def]);
+
+
+val bir_mk_bool_val_inv = store_thm ("bir_mk_bool_val_inv",
+  ``!b. bir_dest_bool_val (bir_mk_bool_val b) = SOME b``,
+Cases >> SIMP_TAC std_ss [bir_mk_bool_val_ALT_DEF_TF, bir_dest_bool_val_TF]);
+
+
+val bir_dest_bool_val_inv = store_thm ("bir_dest_bool_val_inv",
+  ``!b v. (bir_dest_bool_val v = SOME b) ==> (v = bir_mk_bool_val b)``,
+
+REPEAT STRIP_TAC >>
+MP_TAC (Q.SPEC `v` bir_dest_bool_val_EQ_NONE) >>
+ASM_SIMP_TAC std_ss [bir_val_is_Bool_ALT_DEF] >>
+STRIP_TAC >> (
+  FULL_SIMP_TAC std_ss [bir_dest_bool_val_TF, bir_mk_bool_val_ALT_DEF_TF]
+));
+
+
+val bir_dest_bool_val_EQ_SOME = store_thm ("bir_dest_bool_val_EQ_SOME",
+  ``!v b. ((bir_dest_bool_val v) = SOME b) <=>
+          (v = bir_mk_bool_val b)``,
+METIS_TAC[bir_dest_bool_val_inv, bir_mk_bool_val_inv]);
+
+
+val bir_dest_bool_val_IS_SOME = store_thm ("bir_dest_bool_val_IS_SOME",
+  ``!v. IS_SOME (bir_dest_bool_val v) <=>
+        bir_val_is_Bool v``,
+
+GEN_TAC >>
+MP_TAC (Q.SPEC `v` bir_dest_bool_val_EQ_NONE) >>
+Cases_on `bir_dest_bool_val v` >> (
+  ASM_SIMP_TAC std_ss []
+));
+
+
+
+(***********************)
+(* boolean expressions *)
+(***********************)
+
+val bir_exp_true_def  = Define `bir_exp_true  = BExp_Const (Imm1 1w)`;
+val bir_exp_false_def = Define `bir_exp_false = BExp_Const (Imm1 0w)`;
+
+val bir_eval_exp_TF = store_thm ("bir_eval_exp_TF",
+  ``(!env. bir_eval_exp bir_exp_true env = bir_val_true) /\
+    (!env. bir_eval_exp bir_exp_false env = bir_val_false)``,
+
+SIMP_TAC std_ss [bir_exp_false_def, bir_exp_true_def, bir_eval_exp_def,
+  bir_val_true_def, bir_val_false_def]);
+
+
+val bir_is_bool_exp_def = Define `
+  bir_is_bool_exp e <=> (type_of_bir_exp e = SOME (BType_Imm Bit1))`;
+
+val bir_number_of_mem_splits_BitResult = store_thm ("bir_number_of_mem_splits_BitResult",
+  ``!vty aty. bir_number_of_mem_splits vty Bit1 aty =
+              (if vty = Bit1 then SOME 1 else NONE)``,
+
+REPEAT STRIP_TAC >>
+SIMP_TAC std_ss [bir_number_of_mem_splits_def, size_of_bir_immtype_def] >>
+Cases_on `size_of_bir_immtype vty = 1` >- (
+  FULL_SIMP_TAC arith_ss [bitTheory.ONE_LE_TWOEXP,
+    size_of_bir_immtype_EQ_REWRS, size_of_bir_immtype_def]
+) >>
+`size_of_bir_immtype vty <> 0` by METIS_TAC[bir_immTheory.size_of_bir_immtype_NEQ_0] >>
+`1 < size_of_bir_immtype vty` by DECIDE_TAC >>
+ASM_SIMP_TAC arith_ss [] >>
+METIS_TAC[size_of_bir_immtype_def]);
+
+
+val bir_is_bool_exp_REWRS = store_thm ("bir_is_bool_exp_REWRS",
+``(bir_is_bool_exp bir_exp_false) /\
+  (bir_is_bool_exp bir_exp_true) /\
+
+  (!c. (bir_is_bool_exp (BExp_Const c) <=> (type_of_bir_imm c = Bit1))) /\
+
+  (!v. (bir_is_bool_exp (BExp_Den v) <=> (BType_Imm Bit1 = bir_var_type v))) /\
+
+  (!uo e. (bir_is_bool_exp (BExp_UnaryExp uo e) <=> bir_is_bool_exp e)) /\
+
+  (!bo e1 e2. (bir_is_bool_exp (BExp_BinExp bo e1 e2) <=>
+     (bir_is_bool_exp e1 /\ bir_is_bool_exp e2))) /\
+
+  (!bo e1 e2. (bir_is_bool_exp (BExp_BinPred bo e1 e2) <=>
+     ?it. (type_of_bir_exp e1 = SOME (BType_Imm it)) /\
+          (type_of_bir_exp e2 = SOME (BType_Imm it)))) /\
+
+  (!ec e1 e2. (bir_is_bool_exp (BExp_IfThenElse ec e1 e2) <=>
+     bir_is_bool_exp ec /\ bir_is_bool_exp e1 /\ bir_is_bool_exp e2)) /\
+
+  (!ct e s. (bir_is_bool_exp (BExp_Cast ct e s) <=>
+     ((s = Bit1) /\ (?it. (type_of_bir_exp e = SOME (BType_Imm it)))))) /\
+
+  (!ae me en s. (bir_is_bool_exp (BExp_Load ae me en s) <=>
+     ((s = Bit1) /\ (?at.
+     (type_of_bir_exp ae = SOME (BType_Mem at Bit1)) /\
+     (type_of_bir_exp me = SOME (BType_Imm at)))))) /\
+
+  (!ae me ve en. (bir_is_bool_exp (BExp_Store ae me en ve) <=>  F))``,
+
+SIMP_TAC (std_ss++holBACore_ss++boolSimps.EQUIV_EXTRACT_ss) [bir_is_bool_exp_def,
+  bir_exp_true_def, bir_exp_false_def, BType_Bool_def,
+  bir_number_of_mem_splits_BitResult]);
+
+
+
+(*********************************************)
+(* boolean expressions properly typed in env *)
+(*********************************************)
+
+val bir_is_bool_exp_env_def = Define `bir_is_bool_exp_env env e <=>
+  (bir_is_bool_exp e /\
+   (bir_env_vars_are_initialised env (bir_vars_of_exp e)))`;
+
+
+val bir_is_bool_exp_env_IMPLIES_dest_bool_val = store_thm (
+  "bir_is_bool_exp_env_IMPLIES_dest_bool_val",
+  ``!env e. bir_is_bool_exp_env env e ==> bir_is_bool_exp e``,
+SIMP_TAC std_ss [bir_is_bool_exp_env_def]);
+
+
+val bir_is_bool_exp_env_IMPLIES_EVAL_IS_BOOL = store_thm ("bir_is_bool_exp_env_IMPLIES_EVAL_IS_BOOL",
+  ``!env e. bir_is_bool_exp_env env e ==>
+      bir_val_is_Bool (bir_eval_exp e env)``,
+
+SIMP_TAC std_ss [bir_is_bool_exp_env_def, bir_is_bool_exp_def] >>
+REPEAT STRIP_TAC >>
+`type_of_bir_val (bir_eval_exp e env) = SOME (BType_Imm Bit1)` by
+  METIS_TAC[type_of_bir_exp_THM_with_init_vars] >>
+FULL_SIMP_TAC (std_ss++holBACore_ss) [type_of_bir_val_EQ_ELIMS,
+  bir_val_is_Bool_def]);
+
+
+val bir_eval_bool_exp_def = Define `bir_eval_bool_exp env e =
+  THE (bir_dest_bool_val (bir_eval_exp env e))`;
+
+
+
+val bir_eval_bool_exp_INTRO = store_thm ("bir_eval_bool_exp_INTRO",
+  ``!env e. bir_is_bool_exp_env env e ==>
+      (bir_eval_exp e env = bir_mk_bool_val (bir_eval_bool_exp e env))``,
+
+REPEAT STRIP_TAC >>
+`bir_val_is_Bool (bir_eval_exp e env)` by METIS_TAC[bir_is_bool_exp_env_IMPLIES_EVAL_IS_BOOL] >>
+FULL_SIMP_TAC std_ss [bir_eval_bool_exp_def, GSYM bir_dest_bool_val_IS_SOME,
+  optionTheory.IS_SOME_EXISTS] >>
+METIS_TAC[bir_dest_bool_val_inv]);
+
+
+
+
+val bir_is_bool_exp_env_REWRS = store_thm ("bir_is_bool_exp_env_REWRS",
+``(bir_is_bool_exp_env env bir_exp_false) /\
+  (bir_is_bool_exp_env env bir_exp_true) /\
+
+  (!c. (bir_is_bool_exp_env env (BExp_Const c) <=> ((type_of_bir_imm c = Bit1)))) /\
+
+  (!v. (bir_is_bool_exp_env env (BExp_Den v) <=> (
+     bir_env_var_is_initialised env v /\
+     (BType_Imm Bit1 = bir_var_type v)))) /\
+
+  (!uo e. (bir_is_bool_exp_env env (BExp_UnaryExp uo e) <=> bir_is_bool_exp_env env e)) /\
+
+  (!bo e1 e2. (bir_is_bool_exp_env env (BExp_BinExp bo e1 e2) <=>
+     (bir_is_bool_exp_env env e1 /\ bir_is_bool_exp_env env e2))) /\
+
+  (!bo e1 e2. (bir_is_bool_exp_env env (BExp_BinPred bo e1 e2) <=> (
+     bir_env_vars_are_initialised env (bir_vars_of_exp e1) /\
+     bir_env_vars_are_initialised env (bir_vars_of_exp e2) /\
+     ?it. (type_of_bir_exp e1 = SOME (BType_Imm it)) /\
+          (type_of_bir_exp e2 = SOME (BType_Imm it))))) /\
+
+  (!ec e1 e2. (bir_is_bool_exp_env env (BExp_IfThenElse ec e1 e2) <=>
+     bir_is_bool_exp_env env ec /\ bir_is_bool_exp_env env e1 /\ bir_is_bool_exp_env env e2)) /\
+
+  (!ct e s. (bir_is_bool_exp_env env (BExp_Cast ct e s) <=>
+     ((s = Bit1) /\
+     bir_env_vars_are_initialised env (bir_vars_of_exp e) /\
+     (?it. (type_of_bir_exp e = SOME (BType_Imm it)))))) /\
+
+  (!ae me en s. (bir_is_bool_exp_env env (BExp_Load ae me en s) <=>
+     ((s = Bit1) /\
+      bir_env_vars_are_initialised env (bir_vars_of_exp me) /\
+      bir_env_vars_are_initialised env (bir_vars_of_exp ae) /\
+     (?at.
+     (type_of_bir_exp ae = SOME (BType_Mem at Bit1)) /\
+     (type_of_bir_exp me = SOME (BType_Imm at)))))) /\
+
+  (!ae me ve en. (bir_is_bool_exp_env env (BExp_Store ae me en ve) <=>  F))``,
+
+SIMP_TAC (std_ss++holBACore_ss++boolSimps.EQUIV_EXTRACT_ss) [bir_is_bool_exp_env_def,
+  bir_is_bool_exp_REWRS, bir_exp_false_def, bir_exp_true_def,
+  bir_vars_of_exp_def, bir_env_vars_are_initialised_UNION,
+  bir_env_vars_are_initialised_EMPTY, bir_env_vars_are_initialised_INSERT]);
+
+
+
+val bir_eval_bool_exp_TF = store_thm ("bir_eval_bool_exp_TF",
+  ``(!env. (bir_eval_bool_exp bir_exp_true env) = T) /\
+    (!env. (bir_eval_bool_exp bir_exp_false env) = F)``,
+
+SIMP_TAC (std_ss++holBACore_ss) [bir_eval_bool_exp_def, bir_eval_exp_TF,
+  bir_dest_bool_val_TF]);
+
+
+val bir_eval_bool_exp_BExp_Const_bool2b = store_thm ("bir_eval_bool_exp_BExp_Const_bool2b",
+  ``(!env b. (bir_eval_bool_exp (BExp_Const (bool2b b)) env) = b)``,
+
+SIMP_TAC (std_ss++holBACore_ss) [bir_eval_bool_exp_def, GSYM bir_mk_bool_val_def,
+  bir_mk_bool_val_inv]);
+
+
+
+val bir_bin_exp_GET_BOOL_OPER_def = Define
+  `(bir_bin_exp_GET_BOOL_OPER BIExp_And = SOME (T, $/\)) /\
+   (bir_bin_exp_GET_BOOL_OPER BIExp_Or = SOME (T, $\/)) /\
+   (bir_bin_exp_GET_BOOL_OPER BIExp_Xor = SOME (F, (\b1 b2. ~(b1 = b2)))) /\
+   (bir_bin_exp_GET_BOOL_OPER BIExp_Plus = SOME (F, (\b1 b2. ~(b1 = b2)))) /\
+   (bir_bin_exp_GET_BOOL_OPER BIExp_Minus = SOME (F, (\b1 b2. ~(b1 = b2)))) /\
+   (bir_bin_exp_GET_BOOL_OPER BIExp_Mult = SOME (F, $/\ )) /\
+   (bir_bin_exp_GET_BOOL_OPER BIExp_Div = NONE) /\
+   (bir_bin_exp_GET_BOOL_OPER BIExp_SignedDiv = NONE) /\
+   (bir_bin_exp_GET_BOOL_OPER BIExp_Mod =  NONE) /\
+   (bir_bin_exp_GET_BOOL_OPER BIExp_SignedMod = NONE) /\
+   (bir_bin_exp_GET_BOOL_OPER BIExp_LeftShift = SOME (F, \b1 b2. b1 /\ ~b2)) /\
+   (bir_bin_exp_GET_BOOL_OPER BIExp_RightShift = SOME (F, \b1 b2. b1 /\ ~b2)) /\
+   (bir_bin_exp_GET_BOOL_OPER BIExp_SignedRightShift = SOME (F, \b1 b2. b1)) /\
+   (bir_bin_exp_GET_BOOL_OPER _ = NONE) (* Should never fire *)`;
+
+
+val bir_bin_exp_GET_BOOL_OPER_THM = store_thm ("bir_bin_exp_GET_BOOL_OPER_THM",
+  ``!uo de b1 b2 bop. (bir_bin_exp_GET_BOOL_OPER uo = SOME (de, bop)) ==>
+                      (bir_bin_exp uo (bool2b b1) (bool2b b2) =
+                      (bool2b (bop b1 b2)))``,
+
+SIMP_TAC (std_ss++holBACore_ss) [bool2b_def, bir_bin_exp_REWRS] >>
+Cases_on `uo` >> (
+  Cases_on `b1` >> Cases_on `b2` >> (
+    SIMP_TAC (std_ss++boolSimps.LIFT_COND_ss++wordsLib.WORD_ss) [bool2w_def, bir_bin_exp_REWRS,
+      bool2b_def, bir_bin_exp_GET_BOOL_OPER_def, bir_bin_exp_GET_OPER_def]
+  )
+));
+
+
+
+val bir_eval_bool_exp_BExp_BinExp = store_thm ("bir_eval_bool_exp_BExp_BinExp",
+  ``!de uo bop env e1 e2.
+       (bir_bin_exp_GET_BOOL_OPER uo = SOME (de, bop)) ==>
+       bir_is_bool_exp_env env (BExp_BinExp uo e1 e2) ==> (
+       (bir_eval_bool_exp (BExp_BinExp uo e1 e2) env) <=>
+        bop (bir_eval_bool_exp e1 env) (bir_eval_bool_exp e2 env))``,
+
+SIMP_TAC std_ss [bir_eval_bool_exp_def, bir_eval_exp_def, bir_eval_bin_exp_def,
+   bir_is_bool_exp_env_REWRS] >>
+REPEAT STRIP_TAC >>
+`?b1. bir_eval_exp e1 env = bir_mk_bool_val b1` by METIS_TAC[bir_eval_bool_exp_INTRO] >>
+`?b2. bir_eval_exp e2 env = bir_mk_bool_val b2` by METIS_TAC[bir_eval_bool_exp_INTRO] >>
+FULL_SIMP_TAC std_ss [bir_mk_bool_val_inv] >>
+ASM_SIMP_TAC std_ss [bir_eval_bin_exp_def, bir_mk_bool_val_def,
+  type_of_bool2b] >>
+`bir_bin_exp uo (bool2b b1) (bool2b b2) = bool2b (bop b1 b2)` by METIS_TAC[
+   bir_bin_exp_GET_BOOL_OPER_THM] >>
+ASM_SIMP_TAC std_ss [bir_mk_bool_val_inv, GSYM bir_mk_bool_val_def]);
+
+
+val bir_eval_bool_exp_BExp_BinExp_REWRS = save_thm ("bir_eval_bool_exp_BExp_BinExp_REWRS",
+  SIMP_RULE (std_ss++DatatypeSimps.expand_type_quants_ss [``:bir_bin_exp_t``]) [
+    bir_bin_exp_GET_BOOL_OPER_def, bir_is_bool_exp_env_REWRS, FORALL_AND_THM]
+    bir_eval_bool_exp_BExp_BinExp);
+
+val bir_eval_bool_exp_BExp_BinExp_REWRS_GSYM = save_thm ("bir_eval_bool_exp_BExp_BinExp_REWRS_GSYM",
+  GSYM (SIMP_RULE (std_ss++DatatypeSimps.expand_type_quants_ss [``:bir_bin_exp_t``]) [
+    bir_bin_exp_GET_BOOL_OPER_def, bir_is_bool_exp_env_REWRS, FORALL_AND_THM]
+    (SPEC T bir_eval_bool_exp_BExp_BinExp)));
+
+
+
+
+val bir_bin_pred_GET_BOOL_OPER_def = Define
+  `(bir_bin_pred_GET_BOOL_OPER BIExp_Equal = SOME (T, $=)) /\
+   (bir_bin_pred_GET_BOOL_OPER BIExp_NotEqual = SOME (T, $<>)) /\
+   (bir_bin_pred_GET_BOOL_OPER BIExp_LessThan = SOME (F, (\b1 b2. ~b1 /\ b2))) /\
+   (bir_bin_pred_GET_BOOL_OPER BIExp_SignedLessThan = SOME (F, (\b1 b2. b1 /\ ~b2))) /\
+   (bir_bin_pred_GET_BOOL_OPER BIExp_LessOrEqual = SOME (T, $==>)) /\
+   (bir_bin_pred_GET_BOOL_OPER BIExp_SignedLessOrEqual = SOME (F, \b1 b2. b2 ==> b1))`;
+
+
+val bir_bin_pred_GET_BOOL_OPER_THM = store_thm ("bir_bin_pred_GET_BOOL_OPER_THM",
+  ``!uo de b1 b2 bop. (bir_bin_pred_GET_BOOL_OPER uo = SOME (de, bop)) ==>
+                      (bir_bin_pred uo (bool2b b1) (bool2b b2) =
+                      (bop b1 b2))``,
+
+SIMP_TAC (std_ss++holBACore_ss) [bool2b_def, bir_bin_pred_REWRS] >>
+Cases_on `uo` >> (
+  Cases_on `b1` >> Cases_on `b2` >> (
+    SIMP_TAC (std_ss++boolSimps.LIFT_COND_ss++wordsLib.WORD_ss) [bool2w_def, bir_bin_pred_REWRS,
+      bool2b_def, bir_bin_pred_GET_BOOL_OPER_def, bir_bin_pred_GET_OPER_def]
+  )
+));
+
+
+
+val bir_eval_bool_exp_BExp_BinPred = store_thm ("bir_eval_bool_exp_BExp_BinPred",
+  ``!de uo bop env e1 e2.
+       (bir_bin_pred_GET_BOOL_OPER uo = SOME (de, bop)) ==>
+       bir_is_bool_exp_env env e1 ==>
+       bir_is_bool_exp_env env e2 ==> (
+       (bir_eval_bool_exp (BExp_BinPred uo e1 e2) env) <=>
+        bop (bir_eval_bool_exp e1 env) (bir_eval_bool_exp e2 env))``,
+
+SIMP_TAC std_ss [bir_eval_bool_exp_def, bir_eval_exp_def, bir_eval_bin_pred_def,
+   bir_is_bool_exp_env_REWRS] >>
+REPEAT STRIP_TAC >>
+`?b1. bir_eval_exp e1 env = bir_mk_bool_val b1` by METIS_TAC[bir_eval_bool_exp_INTRO] >>
+`?b2. bir_eval_exp e2 env = bir_mk_bool_val b2` by METIS_TAC[bir_eval_bool_exp_INTRO] >>
+FULL_SIMP_TAC std_ss [bir_mk_bool_val_inv] >>
+ASM_SIMP_TAC std_ss [bir_eval_bin_pred_def, bir_mk_bool_val_def,
+  type_of_bool2b] >>
+`bir_bin_pred uo (bool2b b1) (bool2b b2) = bop b1 b2` by METIS_TAC[
+   bir_bin_pred_GET_BOOL_OPER_THM] >>
+ASM_SIMP_TAC std_ss [bir_mk_bool_val_inv, GSYM bir_mk_bool_val_def]);
+
+
+val bir_eval_bool_exp_BExp_BinPred_REWRS = save_thm ("bir_eval_bool_exp_BExp_BinExp_REWRS",
+  SIMP_RULE (std_ss++DatatypeSimps.expand_type_quants_ss [``:bir_bin_pred_t``]) [
+    bir_bin_pred_GET_BOOL_OPER_def, bir_is_bool_exp_env_REWRS, FORALL_AND_THM]
+    bir_eval_bool_exp_BExp_BinPred);
+
+val bir_eval_bool_exp_BExp_BinPred_REWRS_GSYM = save_thm ("bir_eval_bool_exp_BExp_BinExp_REWRS_GSYM",
+  GSYM (SIMP_RULE (std_ss++DatatypeSimps.expand_type_quants_ss [``:bir_bin_pred_t``]) [
+    bir_bin_pred_GET_BOOL_OPER_def, bir_is_bool_exp_env_REWRS, FORALL_AND_THM]
+    (SPEC T bir_eval_bool_exp_BExp_BinPred)));
+
+
+
+val bir_unary_exp_GET_BOOL_OPER_def = Define
+  `(bir_unary_exp_GET_BOOL_OPER BIExp_Not = SOME (T, $~)) /\
+   (bir_unary_exp_GET_BOOL_OPER BiExp_ChangeSign = SOME (F, (\b. b))) /\
+   (bir_unary_exp_GET_BOOL_OPER _ = NONE) (* Should not fire *)`;
+
+
+val bir_unary_exp_GET_BOOL_OPER_THM = store_thm ("bir_unary_exp_GET_BOOL_OPER_THM",
+  ``!de uo b bop. (bir_unary_exp_GET_BOOL_OPER uo = SOME (de, bop)) ==>
+                  (bir_unary_exp uo (bool2b b) = (bool2b (bop b)))``,
+
+SIMP_TAC (std_ss++holBACore_ss) [bool2b_def] >>
+Cases_on `uo` >> (
+  Cases_on `b` >> (
+    SIMP_TAC (std_ss++boolSimps.LIFT_COND_ss++wordsLib.WORD_ss) [bool2w_def,
+      bool2b_def, bir_unary_exp_GET_BOOL_OPER_def, bir_unary_exp_GET_OPER_def]
+  )
+));
+
+
+
+val bir_eval_bool_exp_BExp_UnaryExp = store_thm ("bir_eval_bool_exp_BExp_UnaryExp",
+  ``!de uo bop env e.
+       (bir_unary_exp_GET_BOOL_OPER uo = SOME (de, bop)) ==>
+       bir_is_bool_exp_env env (BExp_UnaryExp uo e) ==> (
+       (bir_eval_bool_exp (BExp_UnaryExp uo e) env) <=>
+        bop (bir_eval_bool_exp e env))``,
+
+SIMP_TAC std_ss [bir_eval_bool_exp_def, bir_eval_exp_def, bir_is_bool_exp_env_REWRS] >>
+REPEAT STRIP_TAC >>
+`?b. bir_eval_exp e env = bir_mk_bool_val b` by METIS_TAC[bir_eval_bool_exp_INTRO] >>
+FULL_SIMP_TAC std_ss [bir_mk_bool_val_inv] >>
+ASM_SIMP_TAC std_ss [bir_eval_unary_exp_def, bir_mk_bool_val_def] >>
+`bir_unary_exp uo (bool2b b) = bool2b (bop b)` by METIS_TAC[
+   bir_unary_exp_GET_BOOL_OPER_THM] >>
+ASM_SIMP_TAC std_ss [bir_mk_bool_val_inv, GSYM bir_mk_bool_val_def]);
+
+
+
+val bir_eval_bool_exp_BExp_UnaryExp_REWRS = save_thm ("bir_eval_bool_exp_BExp_UnaryExp_REWRS",
+  SIMP_RULE (std_ss++DatatypeSimps.expand_type_quants_ss [``:bir_unary_exp_t``]) [
+    bir_unary_exp_GET_BOOL_OPER_def, bir_is_bool_exp_env_REWRS,
+    FORALL_AND_THM]
+    bir_eval_bool_exp_BExp_UnaryExp);
+
+
+val bir_eval_bool_exp_BExp_UnaryExp_REWRS_GSYM = save_thm ("bir_eval_bool_exp_BExp_UnaryExp_REWRS_GSYM",
+  GSYM (SIMP_RULE (std_ss++DatatypeSimps.expand_type_quants_ss [``:bir_unary_exp_t``]) [
+    bir_unary_exp_GET_BOOL_OPER_def, bir_is_bool_exp_env_REWRS,
+    FORALL_AND_THM]
+    (SPEC T bir_eval_bool_exp_BExp_UnaryExp)));
+
+
+
+
+val bir_eval_bool_exp_BExp_IfThenElse = store_thm ("bir_eval_bool_exp_BExp_IfThenElse",
+  ``!env e ec e1 e2.
+       bir_is_bool_exp_env env (BExp_IfThenElse ec e1 e2) ==> (
+       (bir_eval_bool_exp (BExp_IfThenElse ec e1 e2) env) <=>
+        if (bir_eval_bool_exp ec env) then (bir_eval_bool_exp e1 env) else (bir_eval_bool_exp e2 env))``,
+
+SIMP_TAC std_ss [bir_eval_bool_exp_def, bir_eval_exp_def, bir_is_bool_exp_env_REWRS] >>
+REPEAT STRIP_TAC >>
+ASM_SIMP_TAC std_ss [bir_eval_bool_exp_INTRO, bir_mk_bool_val_inv] >>
+SIMP_TAC (std_ss++boolSimps.LIFT_COND_ss) [bir_mk_bool_val_def, bir_eval_ifthenelse_REWRS,
+  type_of_bool2b, bool2b_ELIMS, bool2w_ELIMS] >>
+ASM_SIMP_TAC std_ss [bir_mk_bool_val_inv, GSYM bir_mk_bool_val_def]);
+
+
+val _ = export_theory();
